


\begin{enumerate}[label=\alph*)]
 \item $\vec{a} \cdot \vec{b}=a_xb_x+a_yb_y+a_zb_z=1\cdot(-1)+(-2)\cdot2+3\cdot3=4  $
 \item   $$\vec{a} \cdot \vec{b}=|\vec{a}| \cdot| \vec{b}|\cos\alpha \ \ \ \ \ \Rightarrow  \ \ \ \ \  \cos\alpha=\frac{\vec{a} \cdot \vec{b}}{|\vec{a}| \cdot| \vec{b}|}$$
 $|\vec{a}|=\sqrt{a_x^2+a_y^2+a_z^2}=\sqrt{1^2+(-2)^2+3^2}=\sqrt{14}$
 
 $|\vec{b}|=\sqrt{b_x^2+b_y^2+b_z^2}\sqrt{(-1)^2+2^2+3^2}=\sqrt{14}$
 $$\cos\alpha=\frac{4}{\sqrt{14}\cdot\sqrt{14}} \ \ \ \ \Rightarrow  \ \ \ \  \alpha=\arccos \left( \frac{4}{\sqrt{14} \cdot \sqrt{14}} \right) 
  \ \ \ \ \Rightarrow  \ \ \ \   \alpha=73,4^\circ$$
 
 
 
 \item $\arrowvert \vec{a} \times \vec{b}  \arrowvert =  |\vec{a}| \cdot| \vec{b}|\sin\alpha =\sqrt{14}\cdot\sqrt{14} \sin(73,4^\circ)   $
 $$\arrowvert \vec{a} \times \vec{b}  \arrowvert \approx 13,42$$
 
 
 \item $  \vec{c} =?$
 
 $$\vec{c}=\vec{a} \times \vec{b}=
 \begin{vmatrix}
  \vec{i} & \vec{j} & \vec{k} \\
  a_x  & a_y  & a_z  \\
  b_x  & b_y  & b_z  \\
 \end{vmatrix}
 =\vec{i}(a_yb_z-a_zb_y)-\vec{j}(a_xb_z-a_zb_x) + \vec{k}(a_xb_y-a_yb_x)
 $$
 
 $$\vec{c}=
 \begin{vmatrix}
   \vec{i} & \vec{j} & \vec{k} \\
   1 & -2 & 3 \\
   -1 & 2 & 3 \\
 \end{vmatrix}
 =\vec{i}(-6-6)-\vec{j}(3-(-3))+ \vec{k}(2-2) $$
  $$\vec{c}= -12\vec{i}-6\vec{j} + 0\vec{k}$$
 \item 
 $$\vec{c}= -12\vec{i}-6\vec{j}  \ \ \ \ \Rightarrow  \ \ \ \ |\vec{c}|=\sqrt{144+36} \ \ \ \ \Rightarrow  \ \ \ \ |\vec{c}|\approx13,42 $$
 \item 
 $$\vec{d}=
 \begin{vmatrix}
   \vec{i} & \vec{j} & \vec{k} \\
   -1 & 2 & 3 \\
   1 & -2 & 3 \\
 \end{vmatrix}
 =\vec{i}(6+6)-\vec{j}(-3-3)+ \vec{k}(2-2) $$
  $$\vec{c}= 12\vec{i}+6\vec{j} + 0\vec{k}$$

\end{enumerate}
