
\begin{enumerate}[label=\alph*)]
 \item $h=0$
 $$ E_{p,g}(A) = -\gamma\frac{M_Zm}{R_Z}  $$
 $$  E_{p,g}(A) =- 6,67\cdot  10^{-11}\ Nm^2kg^{-2}\ \frac{5,98 \cdot  10^{24}\ kg\cdot 1 \ kg}{ 6,371 \cdot 10^6\ m}
 = - 62\ 606\ 498,2\ J$$
 $$E_{p,G}=mgh=0\ J $$
 \item $h=10^3\ m$
 $$ E_{p,g}(B) = -\gamma\frac{M_Zm}{R_Z+h}  $$
 $$  E_{p,g}(B) =- 6,67\cdot  10^{-11}\ Nm^2kg^{-2}\ \frac{5,98 \cdot  10^{24}\ kg\cdot 1 \ kg}{ 6,372 \cdot 10^6\ m}
 = - 62\ 596\ 672,9\ J$$
 $$ E_{p,g}(B)- E_{p,g}(A)=9\ 825,3 $$
 $$E_{p,G}=mgh=9\ 810\ J $$
 \item $h=10^6\ m$
 $$ E_{p,g}(C) = -\gamma\frac{M_Zm}{R_Z+h}  $$
 $$  E_{p,g}(C) =- 6,67\cdot  10^{-11}\ Nm^2kg^{-2}\ \frac{5,98 \cdot  10^{24}\ kg\cdot 1 \ kg}{ 6,372 \cdot 10^6\ m}
 = - 54\ 112\ 874,8\ J$$
 $$ E_{p,g}(C)- E_{p,g}(A)=8\ 493\ 623,4 $$
 $$E_{p,G}=mgh=9\ 810\ 000\ J $$
 
 
 
 
\end{enumerate}



